case_study/lean/CaseStudy/Examples/PolarityMepoTest.lean
@@ -1,0 +1,50 @@
+import Hammer
+import CaseStudy.Tactics.Selectors
+
+open Lean LibrarySuggestions
+
+
+set_option trace.auto.tptp.printQuery true
+set_option trace.auto.tptp.result true
+set_option hammer.preprocessingDefault "no_preprocessing"
+set_option hammer.disableAesopDefault true
+set_option hammer.disableGrindDefault true
+set_option hammer.autoPremisesDefault 16
+set_option trace.hammer.premises true
+set_option trace.debug true
+set_option pp.rawOnError true
+set_option trace.mepo true
+
+
+inductive P : Prop
+inductive Q : Prop
+--public theorem p : P := by sorry
+--public theorem p_imp_q : P → Q := by sorry
+
+-- the premises h and h' are irrelevant to the goal
+set_library_suggestions (selectorByName "mepo_polarised").get!
+example : Q := by
+  have h : P := by sorry
+  have h': Q → P := by sorry
+  hammer []
+
+set_library_suggestions mepoSelector (useRarity := false)
+example : Q := by
+  have h : P := by sorry
+  have h': Q → P := by sorry
+  hammer []
+
+
+
+-- the premises h and h' are necessary to prove the goal
+set_library_suggestions (selectorByName "mepo_polarised").get!
+example : Q := by
+  have h : P := by sorry
+  have h': P → Q := by sorry
+  hammer []
+
+set_library_suggestions (selectorByName "mepo").get!
+example : Q := by
+  have h : P := by sorry
+  have h': P → Q := by sorry
+  hammer []
